ECCA/practice.v
@@ -1,0 +1,324 @@
+Require Import core.
+Require Import Coq.micromega.Lia.
+
+Fixpoint trues {V: nat} (e: @exp V): nat:=
+match e with
+  | eId x => 0
+  | eUni U => 0
+  | ePi A B => (trues A) + (trues B)
+  | eAbs A B => (trues A) + (trues B)
+  | eSig A B => (trues A) + (trues B)
+  | ePair v1 v2 A => (trues A) + (trues v1) + (trues v2)
+  | eTru => 1
+  | eFls => 0
+  | eBool => 0
+  | eLet A B => (trues A) + (trues B)
+  | eIf v1 e1 e2 => (trues v1) + (trues e1) + (trues e2)
+  | eApp v1 v2 => (trues v1) + (trues v2)
+  | eFst v => trues v
+  | eSnd v => trues v
+end.
+
+Fixpoint bools {V: nat} (e: @exp V): nat:=
+match e with
+  | eId x => 0
+  | eUni U => 0
+  | ePi A B => (bools A) + (bools B)
+  | eAbs A B => (bools A) + (bools B)
+  | eSig A B => (bools A) + (bools B)
+  | ePair v1 v2 A => (bools A) + (bools v1) + (bools v2)
+  | eTru => 1
+  | eFls => 0
+  | eBool => 0
+  | eLet A B => (bools A) + (bools B)
+  | eIf v1 e1 e2 => (bools v1) + (bools e1) + (bools e2)
+  | eApp v1 v2 => (bools v1) + (bools v2)
+  | eFst v => bools v
+  | eSnd v => bools v
+end.
+
+Goal forall {V: nat}(e:@exp V), trues e <= bools e.
+Proof.
+intros.
+induction e; intuition.
+Qed.
+
+Inductive trues_r {V: nat} : (@exp V) -> nat -> Prop :=
+| t_tru:
+  @trues_r V (eTru) 1
+| t_id (x: atom):
+  @trues_r V (eId x) 0
+| t_uni (U: universe):
+  @trues_r V (eUni U) 0
+| t_fls:
+  @trues_r V eFls 0
+| t_bool:
+  @trues_r V eBool 0
+| t_fst (v: @exp V) (n: nat):
+  trues_r v n ->
+  @trues_r V (eFst v) n
+| t_snd (v: @exp V) (n: nat):
+  trues_r v n ->
+  @trues_r V (eSnd v) n
+| t_pi (A: exp) (B: @exp (S V)) (n3 n4: nat):
+  trues_r A n3 ->
+  @trues_r (S V) B n4 ->
+  @trues_r V (ePi A B) (n3 + n4)
+| t_abs (A: exp) (B: @exp (S V)) (n1 n2: nat):
+  trues_r A n1 ->
+  @trues_r (S V) B n2 ->
+  @trues_r V (eAbs A B) (n1 + n2)
+| t_sig (A: exp) (B: @exp (S V)) (n1 n2: nat):
+  trues_r A n1 ->
+  @trues_r (S V) B n2 ->
+  @trues_r V (eSig A B) (n1 + n2)
+| t_let (A: exp) (B: @exp (S V)) (n1 n2: nat):
+  trues_r A n1 ->
+  @trues_r (S V) B n2 ->
+  @trues_r V (eLet A B) (n1 + n2)
+| t_app (A B: exp) (n1 n2: nat):
+  trues_r A n1 ->
+  @trues_r V B n2 ->
+  @trues_r V (eApp A B) (n1 + n2)
+| t_pair (A v1 v2: exp) (n1 n2 n3: nat):
+  trues_r A n1 ->
+  trues_r v1 n2 ->
+  trues_r v2 n3 ->
+  @trues_r V (ePair v1 v2 A) (n1 + n2 + n3)
+| t_if (v1 e1 e2: exp) (n1 n2 n3: nat):
+  trues_r v1 n1 ->
+  trues_r e1 n2 ->
+  trues_r e2 n3 ->
+  @trues_r V (eIf v1 e1 e2) (n1 + n2 + n3)
+.
+
+Inductive bools_r {V: nat} : (@exp V) -> nat -> Prop :=
+| b_tru:
+  @bools_r V (eTru) 1
+| b_id (x: atom):
+  @bools_r V (eId x) 0
+| b_uni (U: universe):
+  @bools_r V (eUni U) 0
+| b_fls:
+  @bools_r V eFls 1
+| b_bool:
+  @bools_r V eBool 0
+| b_fst (v: @exp V) (n: nat):
+  bools_r v n ->
+  @bools_r V (eFst v) n
+| b_snd (v: @exp V) (n: nat):
+  bools_r v n ->
+  @bools_r V (eSnd v) n
+| b_pi (A: exp) (B: @exp (S V)) (n1 n2: nat):
+  bools_r A n1 ->
+  @bools_r (S V) B n2 ->
+  @bools_r V (ePi A B) (n1 + n2)
+| b_abs (A: exp) (B: @exp (S V)) (n1 n2: nat):
+  bools_r A n1 ->
+  @bools_r (S V) B n2 ->
+  @bools_r V (eAbs A B) (n1 + n2)
+| b_sig (A: exp) (B: @exp (S V)) (n1 n2: nat):
+  bools_r A n1 ->
+  @bools_r (S V) B n2 ->
+  @bools_r V (eSig A B) (n1 + n2)
+| b_let (A: exp) (B: @exp (S V)) (n1 n2: nat):
+  bools_r A n1 ->
+  @bools_r (S V) B n2 ->
+  @bools_r V (eLet A B) (n1 + n2)
+| b_app (A B: exp) (n1 n2: nat):
+  bools_r A n1 ->
+  @bools_r V B n2 ->
+  @bools_r V (eApp A B) (n1 + n2)
+| b_pair (A v1 v2: exp) (n1 n2 n3: nat):
+  bools_r A n1 ->
+  bools_r v1 n2 ->
+  bools_r v2 n3 ->
+  @bools_r V (ePair v1 v2 A) (n1 + n2 + n3)
+| b_if (v1 e1 e2: exp) (n1 n2 n3: nat):
+  bools_r v1 n1 ->
+  bools_r e1 n2 ->
+  bools_r e2 n3 ->
+  @bools_r V (eIf v1 e1 e2) (n1 + n2 + n3)
+.
+
+Lemma boolsr_gte_truesr: forall {V:nat}, forall (e: @exp V) (n1 n2: nat), trues_r e n1 -> bools_r e n2 -> (n2 >= n1).
+Proof. induction e; intros; inversion H; inversion H0; subst; auto.
++ cut (n0 >= n3). cut (n5 >= n4).
+  lia. auto. auto.
++ cut (n4 >= n0). cut (n5 >= n3). lia. auto. auto.
++ cut (n4 >= n0). cut (n5 >= n3). lia. auto. auto.
++ cut (n5 >= n0). cut (n6 >= n3). cut (n7 >= n4). lia. all: auto.
++ cut (n4 >= n0). cut (n5 >= n3). lia. auto. auto.
++ cut (n5 >= n0). cut (n6 >= n3). cut (n7 >= n4). lia. all: auto.
++ cut (n4 >= n0). cut (n5 >= n3). lia. auto. auto.
+Qed.
+
+ Inductive trues_rg : env -> @exp 0 -> nat -> Prop :=
+| t_trug (g: env):
+  trues_rg g (eTru) 1
+| t_idgdef (g: env) (e A: exp) (x: atom) (n: nat):
+  has g x (Def e A) ->
+  trues_rg g e n->
+(*   trues_rg g A n'-> *)
+  trues_rg g (eId x) n
+| t_idgass (g: env) (A: exp) (x: atom) (n: nat):
+  has g x (Assum A) ->
+  trues_rg g A n->
+  trues_rg g (eId x) n
+| t_unig (g: env) (U: universe):
+  trues_rg g (eUni U) 0
+| t_flsg (g: env):
+  trues_rg g eFls 0
+| t_boolg (g: env):
+  trues_rg g eBool 0
+| t_fstg (v: exp) (n: nat) (g: env):
+  trues_rg g v n ->
+  trues_rg g (eFst v) n
+| t_sndg (v: exp) (n: nat) (g: env):
+  trues_rg g v n ->
+  trues_rg g (eSnd v) n
+| t_pig (A: exp) (B: @exp (S 0)) (x: name) (n: nat) (g: env):
+  trues_rg (g & x ~ Assum A) (open x B) n ->
+  trues_rg g (ePi A B) n
+| t_absg (A: exp) (B: @exp (S 0)) (x: name) (n: nat) (g: env):
+  trues_rg (g & x ~ Assum A) (open x B) n ->
+  trues_rg g (eAbs A B) n
+| t_sigg (A: exp) (B: @exp (S 0)) (x: name) (n: nat) (g: env):
+  trues_rg (g & x ~ Assum A) (open x B) n ->
+  trues_rg g (eSig A B) n
+| t_letg (e A: exp) (B: @exp (S 0)) (x: name) (n: nat) (g: env):
+  trues_rg (g & x ~ Def e A) (open x B) n ->
+  trues_rg g (eLet e B) n
+| t_appg (A B: exp) (n1 n2: nat) (g: env):
+  trues_rg g A n1 ->
+  trues_rg g B n2 ->
+  trues_rg g (eApp A B) (n1 + n2)
+| t_pairg (A v1 v2: exp) (n1 n2 n3: nat) (g: env):
+  trues_rg g A n1 ->
+  trues_rg g v1 n2 ->
+  trues_rg g v2 n3 ->
+  trues_rg g (ePair v1 v2 A) (n1 + n2 + n3)
+| t_ifg (v1 e1 e2: exp) (n1 n2 n3: nat) (g: env):
+  trues_rg g v1 n1 ->
+  trues_rg g e1 n2 ->
+  trues_rg g e2 n3 ->
+  trues_rg g (eIf v1 e1 e2) (n1 + n2 + n3) 
+.
+
+Require Import String.
+Open Scope string.
+Goal trues_rg ctx_empty (eLet eTru (eAbs eFls eTru)) 1.
+Proof. eapply t_letg. cbn. eapply t_absg. cbn. eapply t_trug. Unshelve. auto.
+exact "X". exact "Y". Qed.
+
+
+ Inductive bools_rg : env -> @exp 0 -> nat -> Prop :=
+| b_trug (g: env):
+  bools_rg g (eTru) 1
+| b_idgdef (g: env) (e A: exp) (x: atom) (n: nat):
+  has g x (Def e A) ->
+  bools_rg g e n->
+(*   bools_rg g A n'-> *)
+  bools_rg g (eId x) n
+| b_idgass (g: env) (A: exp) (x: atom) (n: nat):
+  has g x (Assum A) ->
+  bools_rg g A n->
+  bools_rg g (eId x) n
+| b_unig (g: env) (U: universe):
+  bools_rg g (eUni U) 0
+| b_flsg (g: env):
+  bools_rg g eFls 1
+| b_boolg (g: env):
+  bools_rg g eBool 0
+| b_fstg (v: exp) (n: nat) (g: env):
+  bools_rg g v n ->
+  bools_rg g (eFst v) n
+| b_sndg (v: exp) (n: nat) (g: env):
+  bools_rg g v n ->
+  bools_rg g (eSnd v) n
+| b_pig (A: exp) (B: @exp (S 0)) (x: name) (n: nat) (g: env):
+  bools_rg (g & x ~ Assum A) (open x B) n ->
+  bools_rg g (ePi A B) n
+| b_absg (A: exp) (B: @exp (S 0)) (x: name) (n: nat) (g: env):
+  bools_rg (g & x ~ Assum A) (open x B) n ->
+  bools_rg g (eAbs A B) n
+| b_sigg (A: exp) (B: @exp (S 0)) (x: name) (n: nat) (g: env):
+  bools_rg (g & x ~ Assum A) (open x B) n ->
+  bools_rg g (eSig A B) n
+| b_letg (e A: exp) (B: @exp (S 0)) (x: name) (n: nat) (g: env):
+  bools_rg (g & x ~ Def e A) (open x B) n ->
+  bools_rg g (eLet e B) n
+| b_appg (A B: exp) (n1 n2: nat) (g: env):
+  bools_rg g A n1 ->
+  bools_rg g B n2 ->
+  bools_rg g (eApp A B) (n1 + n2)
+| b_pairg (A v1 v2: exp) (n1 n2 n3: nat) (g: env):
+  bools_rg g A n1 ->
+  bools_rg g v1 n2 ->
+  bools_rg g v2 n3 ->
+  bools_rg g (ePair v1 v2 A) (n1 + n2 + n3)
+| b_ifg (v1 e1 e2: exp) (n1 n2 n3: nat) (g: env):
+  bools_rg g v1 n1 ->
+  bools_rg g e1 n2 ->
+  bools_rg g e2 n3 ->
+  bools_rg g (eIf v1 e1 e2) (n1 + n2 + n3) 
+.
+
+Eval simpl in (has (ctx_empty & "X" ~ eBool) (free "X") eTru).
+
+Lemma nothing_in_empty: forall {A}(x: @var 0) M, ((@ctx_empty A) ∋ x ~ M) = False.
+Proof.
+intros. cbn. reflexivity. Qed.
+Require Import Coq.Program.Equality.
+
+Lemma has_function {A} (g: @context A)(x: var) (M M': A): 
+has g x M /\ has g x M' ->
+M = M'.
+Proof.
+intros. destruct H. dependent induction g.
++ cbn in H. contradiction. 
++ cbn in H. cbn in H0. destruct (bindv (closev a x)).
+  - apply IHg with (x:= v). auto. auto. 
+  - subst. reflexivity.
+Qed.
+
+Require Import Coq.Program.Equality.
+Lemma boolsrg_gte_truesrg: forall (g: env) (e: @exp 0)  (n1 n2: nat), trues_rg g e n1 -> bools_rg g e n2 -> (n2 >= n1).
+Proof. intros.
+dependent induction g; dependent induction e.
+  - inversion H; inversion H0; subst; cbn in *; try contradiction.
+  - inversion H; inversion H0; subst. auto.
+  - inversion H; inversion H0; subst.
+
++ inversion H; inversion H0; subst; cbn in *; try contradiction.
++ inversion H; inversion H0; subst.
+  - cut ((Def e A) = (Def e0 A0)).
+    * intro. inversion H1. subst. 
+    * apply has_function with (x0:=x) (g0:=g). auto. 
+
+
+
+ 
+
+
+
+
+
+
+inversion H; inversion H0; subst; try lia; try discriminate. 
++ inversion H9. subst. cbn. 
+ dependent induction e.
++ intros. inversion H; inversion H0. subst. 
+  - 
++ cut (n0 >= n3). cut (n5 >= n4).
+  lia. auto. auto.
++ cut (n4 >= n0). cut (n5 >= n3). lia. auto. auto.
++ cut (n4 >= n0). cut (n5 >= n3). lia. auto. auto.
++ cut (n5 >= n0). cut (n6 >= n3). cut (n7 >= n4). lia. all: auto.
++ cut (n4 >= n0). cut (n5 >= n3). lia. auto. auto.
++ cut (n5 >= n0). cut (n6 >= n3). cut (n7 >= n4). lia. all: auto.
++ cut (n4 >= n0). cut (n5 >= n3). lia. auto. auto.
+Qed.
+
+
+
