ECCA/typing.v
@@ -52,7 +52,7 @@ Inductive Types: env -> exp -> exp -> Prop :=
   (g |- (eFls) : (eBool)) 
 | aT_Sig (g: env) (x: name) (A B: exp) (i: nat) :
   (g |- A : (eUni (uType i))) ->
-  (Types (g & x ~ Assum A) (open x B) (eUni (uType i))) ->
+  ((g & x ~ Assum A) |- (open x B): (eUni (uType i))) ->
   (g |- (eSig A B) : (eUni (uType i)))
 | aT_Pair (g: env) (v1 v2: exp) (A B: exp) :
   (g |- v1 : A) ->
@@ -74,10 +74,10 @@ Inductive Types: env -> exp -> exp -> Prop :=
   (Types (g & x ~ Def n A) (open x m) (open x B)) ->
   (g |- (eLet n m) : (bind n B))
 | aT_If (g: env) (B U e1 e2: exp) (e: exp) (x y: name):
-  Types (g & x ~ Assum eBool) (open x B) U -> 
-  Types g e eBool ->
-  Types (g & y ~ Eq e eTru) e1 (bind eTru B) ->
-  Types (g & y ~ Eq e eFls) e2 (bind eFls B) -> 
+  ((g & x ~ Assum eBool) |- (open x B): U) -> 
+  (g |- e : eBool) ->
+  ((g & y ~ Eq e eTru) |- e1 : (bind eTru B)) ->
+  ((g & y ~ Eq e eFls) |- e2 : (bind eFls B)) -> 
   (g |- (eIf e e1 e2) : (bind e B)) 
 | aT_Conv (g: env) (e A B U: exp) :
   (g |- e : A) ->
@@ -98,13 +98,13 @@ where "g '|-' a ':' b" := (Types g a b) : ECCA_scope
 with 
 (* ECCA Well-Formed Environments *)
 WellFormed: env -> Prop :=
-| W_Empty (g: @env 0) :
+| wf_Empty:
   WellFormed ctx_empty
-| W_Assum (g: env) (x: name) (A U: exp) :
+| wf_Assum (g: env) (x: name) (A U: exp) :
   WellFormed g ->
   Types g A U ->
   WellFormed (g & x ~ Assum A)
-| W_Def (g: env) (x: name) (e A U: exp) :
+| wf_Def (g: env) (x: name) (e A U: exp) :
   WellFormed g ->
   Types g A U ->
   Types g e A ->
@@ -118,63 +118,63 @@ Well boundedness wrt Type Environments
 =====================================
 *)
 
-Inductive WellBound {V: nat}: env -> exp -> Prop :=
-| wf_Prop (g: env) :
+Inductive WellBound: env -> @exp 0 -> Prop :=
+| wb_Prop (g: env) :
     WellFormed g ->
     WellBound g (eUni uProp)
-| wf_Type (g: env) (i: nat) :
+| wb_Type (g: env) (i: nat) :
     WellFormed g ->
     WellBound g (eUni (uType i))
-| wf_Var (g: env) (x: atom) (A: exp) :
+| wb_Var (g: env) (x: atom) (A: exp) :
     (assumes g x A) -> (* this needs adjustment *)
     WellBound g (eId x)
-| wf_Bool (g: env) :
+| wb_Bool (g: env) :
     WellFormed g ->
     WellBound g eBool
-| wf_True (g: env):
+| wb_True (g: env):
     WellFormed g ->
     WellBound g eTru
-| wf_False (g: env):
+| wb_False (g: env):
     WellFormed g ->
     WellBound g eFls
-| wf_Sig (g: env) (x: name) (A B: exp) (i: nat) :
+| wb_Sig (g: env) (x: name) (A B: exp) (i: nat) :
     WellBound g A ->
     WellBound (g & x ~ Assum A) (open x B) ->
     WellBound g (eSig A B)
-| wf_Pair (g: env) (v1 v2: exp) (A B: exp) (x: name) :
+| wb_Pair (g: env) (v1 v2: exp) (A B: exp) (x: name) :
     WellBound g v1 ->
     WellBound g v2 ->
     WellBound g A ->
     WellBound (g & x ~ Def v1 A) (open x B) ->
     WellBound g (ePair v1 v2 (eSig A B))
-| wf_Pi (g: env) (x: name) (A B: exp) :
+| wb_Pi (g: env) (x: name) (A B: exp) :
     WellBound g A ->
     WellBound (g & x ~ Assum A) (open x B) ->
     WellBound g (ePi A B)
-| wf_Lam (g: env) (x: name) (A e B: exp) :
+| wb_Lam (g: env) (x: name) (A e B: exp) :
     WellBound (g & x ~ Assum A) (open x B) ->
     WellBound (g & x ~ Assum A) (open x e) ->
     WellBound g (eAbs A e)
-| wf_Let (g: env) (n m A B: exp) (x: name):
+| wb_Let (g: env) (n m A B: exp) (x: name):
     WellBound g n ->
     WellBound g A ->
     WellBound (g & x ~ Def n A) (open x B) ->
     WellBound (g & x ~ Def n A) (open x m) ->
     WellBound g (eLet n m)
-| wf_If (g: env) (B e1 e2: exp) (e: exp) (x y: name):
+| wb_If (g: env) (B e1 e2: exp) (e: exp) (x y: name):
     WellBound (g & x ~ Assum eBool) (open x B) -> 
     WellBound g e ->
     WellBound (g & y ~ Eq e eTru) e1 ->
     WellBound (g & y ~ Eq e eFls) e2 -> 
     WellBound g (eIf e e1 e2)
-| wf_App (g: env) (x: name) (e e': exp):
+| wb_App (g: env) (x: name) (e e': exp):
     WellBound g e ->
     WellBound g e' ->
     WellBound g (eApp e e')
-| wf_Fst (g: env) (e: exp) :
+| wb_Fst (g: env) (e: exp) :
     WellBound g e ->
     WellBound g (eFst e)
-| wf_Snd (g: env) (e: exp) :
+| wb_Snd (g: env) (e: exp) :
     WellBound g e ->
     WellBound g (eSnd e)
 .
@@ -203,20 +203,20 @@ comp {V: nat}: Type :=
   | Snd (v: val)
 .*)
 
-Inductive WellBound_val {V: nat}: @env 0 -> val -> Prop :=
-| wf_val_Id (g: env) (A: exp) (x: atom):
+Inductive WellBound_val: env -> @val 0 -> Prop :=
+| wb_val_Id (g: env) (A: exp) (x: atom):
     (assumes g x A) -> (* this needs adjustment *)
     WellBound_val g (Id x)
-| wf_val_Prop (g: env) :
+| wb_val_Prop (g: env) :
     WellFormed g ->
     WellBound_val g (Uni uProp)
-| wf_val_Type (g: env) (i: nat) :
+| wb_val_Type (g: env) (i: nat) :
     WellFormed g ->
     WellBound_val g (Uni (uType i))
-| wf_val_Bool (g: env) :
+| wb_val_Bool (g: env) :
     WellFormed g ->
     WellBound_val g Bool
-| wf_val_True (g: env):
+| wb_val_True (g: env):
     WellFormed g ->
     WellBound_val g Tru
 | wf_val_False (g: env):
@@ -239,7 +239,7 @@ Inductive WellBound_val {V: nat}: @env 0 -> val -> Prop :=
 | wf_val_Lam (g: env) (x: name) (A e: conf) :
     WellBound_conf (g & x ~ Assum (unrestrict_conf A)) (open_conf x e) ->
     WellBound_val g (Abs A e)
-with WellBound_conf {V: nat}: env -> conf -> Prop :=  
+with WellBound_conf: env -> @conf 0 -> Prop :=  
 | wf_conf_Comp (g: env) (e: comp):
     WellBound_comp g e ->
     WellBound_conf g (Comp e)
@@ -254,7 +254,7 @@ with WellBound_conf {V: nat}: env -> conf -> Prop :=
     WellBound_conf (g & y ~ Eq (unrestrict_val v) eTru) m1 ->
     WellBound_conf (g & y ~ Eq (unrestrict_val v) eFls) m2 -> 
     WellBound_conf g (If v m1 m2)
-with WellBound_comp {V: nat}: env -> comp -> Prop :=
+with WellBound_comp: env -> @comp 0 -> Prop :=
 | wf_comp_Val (g: env) (v: val):
     WellBound_val g v ->
     WellBound_comp g (Val v)
